Update end-to-end correctness proofs for parse table generation pipeline

LL1/ParseTableGen.v
@@ -213,7 +213,8 @@ Definition mkParseTable (ps : list table_entry) : option parse_table :=
 (* Combining all of the steps into a single function *)
 (* The type of this function will change as I add code for computing NULLABLE, etc. *)
 
-Definition genTableForGrammar g nu fi fo :=
+Definition genTableForGrammar g fi fo :=
+  let nu := mkNullableSet g in
   let es := mkEntries nu fi fo g in
   mkParseTable es.
 
